Connect/Common.v
@@ -20,18 +20,14 @@
 
 Require Import String.
 Require Import Ascii.
-Require Import List.
-Require Import ListSet.
 Require Import EqNat.
-Import ListNotations.
 Require Import Arith.
-Open Scope list_scope.
-Fixpoint len {T:Type}(x : list T) : nat :=
-  match x with
-    | x::b => 1+len b
-    | nil => 0
-  end.
-Fixpoint suml (x : list nat) : nat :=
+
+Require Import Vector.
+Import Vector.
+Import VectorNotations.
+Fixpoint len {n} {T:Type}(x : Vector.t T n) : nat := n.
+Fixpoint suml {n} (x : Vector.t nat n) : nat :=
   match x with
     | x::b => x+suml b
     | nil => 0
