Connect/c8051.v
@@ -69,13 +69,17 @@ Definition r := {|
 Module i8051_Component.
   (* Variable threshold : nat. *)
   Definition threshold := 1.
-  Search nat.
-  Definition digitizer : IO.func 1:=
-    (fun x =>
-                    match threshold - (hd 0 (Vector.hd  x)) with
+  Definition tighter {n} (x : Vector.t (Vector.t IO.t (S n)) 1) threshold := 
+                    match threshold - (Vector.hd (Vector.hd  x)) with
                       | 0 => 1
                       | _ => 0
-                    end).
+                    end.
+  Definition digitizer : IO.func 1:=
+    fun c=>  (fun x =>  
+                match x with
+                  | (Vector.cons  (Vector.cons r _ l) 0 Vector.nil) as V  => tighter V threshold
+                  | _ => 0
+                end).
   Fixpoint digitize l acc :=
     match l with
       | (a, b) :: r => digitize r (acc // a ~> digitizer  ~> b # b ("Digitized Port"))
@@ -86,7 +90,7 @@ Module i8051_Component.
 
   
 
-  Definition run_8051 init ps := dump_state  {|
+  Definition run_8051 { c} init (ps:Vector.t ports c) := Run8051.dump_state  {|
                                                     rtl_oracle :=  {|
                                                                    oracle_bits := Word.repr ; 
                                                                    oracle_offset := 0
@@ -103,10 +107,8 @@ Module i8051_Component.
   (*                              | None => nil *)
   (*                            end) init in *)
   (*  run8051 cycle  (load_code_bytes loads). *)
-  Definition run_8051_bin_string bin ps := 
+  Definition run_8051_bin_string {c} bin (ps:Vector.t ports c) := 
     run_8051 (load_code_bytes_bin bin 0) ps.
-  SearchAbout nat.
-  SearchAbout Word.int.
   Definition condense (b7 b6 b5 b4 b3 b2 b1 b0: bool) :=
     let i7 : int8 := Word.bool_to_int b7 in
     let i6 : int8 := Word.bool_to_int b6 in
@@ -118,48 +120,149 @@ Module i8051_Component.
     let i0 : int8 := Word.bool_to_int b0 in
     fold_left (fun s f => Word.or (Word.shl s (Word.repr 1))  f) [i7;i6;i5;i4;i3;i2;i1;i0] Word.zero.
 
-  Fixpoint condense' l7 l6 l5 l4 l3 l2 l1 l0 :=
-    match l7, l6, l5, l4, l3, l2, l1, l0  with
-        | a::a',b::b',c::c',d::d',e::e',f::f',g::g',h::h' => (condense a b c d e f g h) :: (condense' a' b' c' d' e' f' g' h')
-        | _,_,_,_,_,_,_,_ => []
-    end.
-  
-  Fixpoint to_trace p1 p2 p3 p4 :=
-    match p1, p2, p3, p4 with
-      | a::a', b::b', c::c', d::d' => {| P0 := a; P1 := b; P2:=c;P3:=d |} :: to_trace a' b' c' d'
-      | _,_,_,_ => []
-    end.
-
   Require Import Vector.
   Import VectorNotations.
   Import Vector.
-  Require Import Fin.
-  Import Fin.
-  Close Scope vector_scope.
-  Open  Scope list_scope.
-  Definition traces (tr:Vector.t (list nat) 32) thresh :=
-    let f := Vector.map (List.map (fun x => NPeano.ltb x thresh)) in
-    let digitized := to_list( f tr) in
+  Definition map {A} {B} (f : A -> B) : forall {n} (v:t A n), t B n :=
+    fix map_fix {n} (v : t A n) : t B n := match v with
+                                             | [] => []
+                                             | a :: v' => (f a) :: (map_fix v')
+                                           end.
+
+  (* Definition map {A} {B} (f : A->A->A->A->A->A->A->A -> B) : *)
+  (*   forall {n} (l7 l6 l5 l4 l3 l2 l1 l0: t A n), t B n := *)
+  (*   fix map_fix {n} (l7 l6 l5 l4 l3 l2 l1 l0 : t A n) : t B n := *)
+  (*   match l7, l6, l5, l4, l3, l2, l1, l0  with *)
+  (*     | a::a',b::b',c::c',d::d',e::e',f::f',g::g',h::h' => *)
+  (*       (f a b c d e f g h) :: (map_fix a' b' c' d' e' f' g' h') *)
+  (*     | _,_,_,_,_,_,_,_ => [] *)
+  (*   end. *)
+
+  (*   match v with *)
+  (*                                            | [] => [] *)
+  (*                                            | a :: v' => (f a) :: (map_fix v') *)
+  (*                                          end. *)
+
+      (* | a::b::c::d::e::f::g::h::i::j => I *)
+      (* | a::b::c::d::e::f::g::[] => I *)
+      (* | a::b::c::d::e::f::[]=> I *)
+      (* | a::b::c::d::e::[] => I *)
+      (* | a::b::c::d::[] => I *)
+      (* | a::b::c::[] => I *)
+      (* | a::b::[] => I *)
+      (* | a::[] => I *)
+  Check ([1]).
+  Definition get8th {A} (v:Vector.t A 8) : A:=
+    hd (tl (tl (tl (tl (tl (tl (tl v))))))).
+  Definition get7th {A} (v:Vector.t A 8) : A:=
+    hd (tl (tl (tl (tl (tl (tl v)))))).
+  Definition get6th {A} (v:Vector.t A 8) : A:=
+    hd (tl (tl (tl (tl (tl v))))).
+
+  Definition get5th {A} (v:Vector.t A 8) : A:=
+    hd  (tl (tl (tl (tl v)))).
+
+  Definition get4th {A} (v:Vector.t A 8) : A:=
+    hd  (tl (tl (tl v))).
+
+  Definition get3rd {A} (v:Vector.t A 8) : A:=
+    hd  (tl (tl v)).
+
+  Definition get2nd {A} (v:Vector.t A 8) : A:=
+    hd  (tl v).
+
+  Definition get1st {A} (v:Vector.t A 8) : A:=
+    hd  v.
+  Definition condense' {n} (v' : Vector.t (Vector.t bool n) 8) :=  (* Vector.t int8 n:= *)
+
+    let v2 := Vector.map (Vector.map (fun f:bool => if f then Word.one else @Word.zero 7)) v' in
+    let v := Vector.map2 (fun f1 f2 => Vector.map (fun f => Word.shl f (Word.repr (Z_of_nat f2))) f1) v2 (of_list (seq 0 8)) in
+    (* match v  in Vector.t _ n' return ( match  n'  with *)
+    (*                                     |0 => unit *)
+    (*                                     |1=>unit *)
+    (*                                     |2 => unit *)
+    (*                                     |3=> unit *)
+    (*                                     |4=> unit *)
+    (*                                     |5=> unit *)
+    (*                                     | 6 => unit *)
+    (*                                     |7 => unit *)
+    (*                                     | S(S(S(S(S(S(S(S(S n)))))))) => unit *)
+    (*                                     | 8 => Vector.t int8 n' *)
+    (*                                      end) with *)
+    (*   | [] => tt   *)
+    (*   | [_] => tt   *)
+    (*   | [_;_;_] => tt   *)
+    (*   | [_;_;_;_] => tt   *)
+    (*   | [_;_;_;_;_] => tt   *)
+    (*   | [_;_;_;_;_;_] => tt   *)
+    (*   | [_;_;_;_;_;_;_] => tt   *)
+    (*   | [_;_;_;_;_;_;_;_] => tt   *)
+    (*   | a::b::c::d::e::f::g::h::i::_ => a *)
+    (*   | a::b::c::d::e::f::g::h::[] => a *)
+    (*   end. *)
+    let l7 := get8th v in
+    let l6 := get7th v in
+    let l5 := get6th v in
+    let l4 := get5th v in
+    let l3 := get4th v in
+    let l2 := get3rd v in
+    let l1 := get2nd v in
+    let l0 := get1st v in
+    let or := Vector.map2 (fun f1 f2 => Word.or f1 f2) in
+    let a0 := or l0 l1 in
+    let a1 := or l2 l3 in
+    let a2 := or l4 l5 in
+    let a3 := or l6 l7 in
+    let a4 := or a0 a1 in
+    let a5 := or a2 a3 in
+    or a4 a5 .
+
+
+
+  (* match v  as f in (Vector.t _ eight) *)
+  (*         return (match  eight with *)
+  (*                   | 8 => Vector.t int8 n *)
+  (*                   | _ => True *)
+  (*                 end) with *)
+  (*     (* | [a::a';b::b';c::c';d::d';e::e';f::f';g::g';h::h'] => *) *)
+  (*     (*   (* Vector.nil int8 *) *) *)
+  (*     (*   (condense a b c d e f g h)::(condense' a' b' c' d' e' f' g' h') *) *)
+  (*     (* | a::b::c::d::e::f::g::h::[] => Vector.nil int8 *) *)
+  (*     | map *)
+  (*     | _ => I *)
+  (*   end. *)
+  
+  Fixpoint to_trace {n} (p0 p1 p2 p3: Vector.t int8 n) :=
+    let m := Vector.map2
+               (fun p0 p1 => {| P0 := p0; P1 := p1; P2:=Word.zero;P3:=Word.zero |}) p0 p1 in 
+    let m' := Vector.map2 (fun p2 m' => {| P0 := P0 m'; P1 := P1 m'; P2:=p2;P3:= Word.zero |}) p2 m in
+    Vector.map2 (fun p3 m'' => {| P0 := P0 m''; P1 := P1 m''; P2:=P2 m'';P3:= p3 |}) p3 m'.
+
+  Definition traces {c} (tr:Vector.t (Vector.t IO.t c) 32) thresh :=
+    let f := Vector.map (Vector.map (fun x => NPeano.ltb x thresh)) in
+    let digitized := ( f tr) in
     
 
     match digitized with
         |(p00::p01::p02::p03::p04::p05::p06::p07::
            p10::p11::p12::p13::p14::p15::p16::p17::
            p20::p21::p22::p23::p24::p25::p26::p27::
-           p30::p31::p32::p33::p34::p35::p36::p37::List.nil) =>
+           p30::p31::p32::p33::p34::p35::p36::p37::[]) =>
          
-        to_trace (condense' p07 p06 p05 p04 p03 p02 p01 p00)
-         (condense' p17 p16 p15 p14 p13 p12 p11 p10)
-         (condense' p27 p26 p25 p24 p23 p22 p21 p20)
-         (condense' p37 p36 p35 p34 p33 p32 p31 p30)
-        |_ => List.nil
+        to_trace (condense' [p07;p06; p05; p04; p03; p02; p01; p00])
+         (condense' [p17; p16; p15; p14; p13; p12; p11; p10])
+         (condense' [p27; p26; p25; p24; p23; p22; p21; p20])
+         (condense' [p37; p36; p35; p34; p33; p32; p31; p30] )
+         (* How can I show this term irrelevant? *)
+        |_ => Vector.const {| P0:=Word.zero ; P1 := Word.zero; P2 := Word.zero; P3 := Word.zero |} c
     end.
         
 
     
 
     
-  Definition i8051_Component bin threshold (conv: option ports -> nat):= (fun t =>
+  Definition i8051_Component bin threshold (conv: option ports -> nat):=
+    fun c:nat => (fun t:Vector.t (Vector.t IO.t c) 32 =>
                      let ps := traces t threshold in
                      conv (run_8051_bin_string bin ps)).
   
@@ -167,15 +270,10 @@ Module i8051_Component.
   Definition conv_char (c:ascii) : int8 := Word.repr (Z_of_nat (nat_of_ascii c)).
 Check i8051_Component.
 End i8051_Component.
-Compute (seq 0 32).
 Import i8051_Component.
-SearchAbout Word.int.
-Check Z.to_N.
-Search nat.
 Definition dac x := match x with
 					  | Some v =>
 						let z := P3 v in
 						N.to_nat(    Z.to_N (Word.unsigned (Word.and z (Word.not (Word.repr 1)))))
                       | None => 0
                     end.
-Check dac.
